closures/Types.v
@@ -1,0 +1,88 @@
+(** * Types as closures *)
+
+Require Import ObAxioms.
+Require Import Lambda.
+Require Import Constructor.
+
+Open Local Scope Ob_scope.
+
+(** ** Properties of types *)
+
+Definition closure (a : Ob) := I [= a /\ a o a = a.
+Definition fixes (a : Ob) (x : Ob) := a*x = x.
+Notation "x :: a" := (fixes a x) : Ob_scope.
+
+(** ** Atomic types *)
+
+Lemma I_closure: closure I.
+Proof.
+  unfold closure; split.
+  apply LESS_refl.
+  apply extensionality.
+  (* TODO *)
+Admitted.
+
+Theorem I_inhab (x : Ob) : x :: I <-> True.
+Proof.
+  (* TODO *)
+Admitted.
+
+Lemma V_closure: closure V.
+Proof.
+  (* TODO *)
+Admitted.
+
+Theorem V_inhab (x : Ob) : x :: V <-> closure x.
+Proof.
+  (* TODO *)
+Admitted.
+
+Corollary fixes_V_V: fixes V V.
+Proof.
+  apply V_inhab.
+  apply V_closure.
+Qed.
+
+Section semi.
+  Local Open Scope Lambda_scope.
+  Let a := VAR 0.
+  Let a' := VAR 1.
+  Definition semi := encode (\\a,a'; a --> a').
+End semi.
+
+Lemma semi_closure: closure semi.
+Proof.
+  (* TODO *)
+Admitted.
+
+Theorem semi_inhab (x : Ob) : x :: semi <->
+  x = BOT \/
+  x = I \/
+  x = TOP.
+Proof.
+  split.
+  (* TODO *)
+Admitted.
+
+Section boool.
+  Local Open Scope Lambda_scope.
+  Let a := VAR 0.
+  Let a' := VAR 1.
+  Definition boool := encode (\\a,a'; a --> a --> a').
+End boool.
+
+Lemma boool_closure: closure semi.
+Proof.
+  (* TODO *)
+Admitted.
+
+Theorem boool_inhab (x : Ob) : x :: boool <->
+  x = BOT \/
+  x = K \/
+  x = F \/
+  x = J \/
+  x = TOP.
+Proof.
+  split.
+  (* TODO *)
+Admitted.
